code/experimental/pkcs/Hacl.Impl.PKCS11.External.DER.fst
@@ -1,0 +1,40 @@
+module Hacl.Impl.PKCS11.External.DER
+
+open FStar.HyperStack.All
+open FStar.HyperStack
+module ST = FStar.HyperStack.ST
+
+open Lib.IntTypes
+
+open Hacl.Impl.PKCS11.Internal.Types
+open Hacl.Impl.PKCS11.Result
+
+open LowStar.Buffer
+open Lib.RawIntTypes
+
+
+assume val getCurveIdentifier: ulCount: size_t -> p: buffer uint8 {length p == uint_v ulCount /\ length p >=3} ->
+  Stack ((e: exception_t) & (_HACL_Curve_ID))
+  (requires fun h -> True)
+  (ensures fun h0 _ h1 -> True)
+  
+
+(* to change to another exception, the curve not supported is ONLY when the parsing was successful, but indeed not supported *)
+
+(* https://en.wikipedia.org/wiki/X.690 *)
+val parseEC_ANSI_962: ulCount: size_t -> p: buffer uint8 {length p == uint_v ulCount /\ length p >=3 } ->
+  Stack ((e: exception_t) & (_HACL_Curve_ID))
+  (requires fun h -> True)
+  (ensures fun h0 _ h1 -> True)
+
+let parseEC_ANSI_962 ulCount p = 
+  let expectedLength = to_u32 (index p 2ul) in 
+  let sizeToCompare = ulCount - 2 in 
+  if expectedLength <> sizeToCompare then 
+    (|CKR_CURVE_NOT_SUPPORTED, 0ul|)
+  else
+    let objectIdentifier = to_u8 (index p 1ul) in 
+      if objectIdentifier <> 9ul then 
+	(|CKR_CURVE_NOT_SUPPORTED, 0ul|)
+      else
+	getCurveIdentifier ulCount p
